Working on `from_bytes_be`

src/LeanEVM/Byte.lean
@@ -5,19 +5,27 @@ def byte := Fin 256
 
 opaque BYTE_0 : byte := {val:=0, isLt:=(by simp)}
 
--- Construct a natural number from a sequence of one or more bytes store in big
+-- Construct a natural number from a sequence of one or more bytes stored in big
 -- endian form.
-def from_bytes_be(bytes:List byte)(i: Fin bytes.length) : Nat :=
-  match bytes, i with
-  | b::_, {val:=0,isLt:=_} => b.val
-  | b::bs, {val:=k+1,isLt:=p} =>
-      have q : k < bs.length := by exact Nat.succ_lt_succ_iff.mp p
-      let im1 : Fin bs.length := {val:= k, isLt:=by exact q}
-      (256 * (from_bytes_be bs im1)) + b.val
+def from_bytes_be(bytes:List byte) : Nat :=
+  match bytes with
+  | List.nil => 0
+  | b::bs =>
+      (256 * (from_bytes_be bs)) + b.val
+
+-- Bound size of number returned by `from_bytes_be`.
+lemma from_bytes_be_bound(n:Nat)(bytes:List byte)(p:bytes.length ≤ n) : (from_bytes_be bytes) < 256^n :=
+by
+  match bytes with
+  | List.nil => unfold from_bytes_be; simp
+  | b::bs =>
+      have p := from_bytes_be_bound n bs
+      unfold from_bytes_be
+      --unfold List.length
+      sorry
 
 -- Prove that converting an array consisting of a single byte generates the
 -- corresponding Nat.
-example (n:byte)(i:Fin 1): (from_bytes_be [n] i) = n.val :=
+example (n:byte): (from_bytes_be [n]) = n.val :=
 by
-  match i with
-  | 0 => rfl
+  repeat unfold from_bytes_be; simp
