src/LeanEVM/Eval.lean
@@ -54,14 +54,14 @@ by
   simp
 
 -- Executing DUP1 has the right effect
-example (evm:Evm): ∃evm', (eval [Push n, Dup_1] evm) = (Ok evm') :=
+example (evm:Evm): ∃evm', (eval [Push ns, Dup_1] evm) = (Ok evm') :=
 by
   let n := u256.from_bytes ns;
   exists {stack := n::n::evm.stack}
   simp [*]
 
 -- Executing DUP2 has the right effect
-example (evm:Evm): ∃evm', (eval [Push n, Push m, Dup_2] evm) = (Ok evm') :=
+example (evm:Evm): ∃evm', (eval [Push ns, Push ms, Dup_2] evm) = (Ok evm') :=
 by
   let n := u256.from_bytes ns;
   let m := u256.from_bytes ms;
@@ -69,7 +69,7 @@ by
   simp [*]
 
 -- Executing DUP3 has the right effect
-example (evm:Evm): ∃evm', (eval [Push n, Push m, Push l, Dup_3] evm) = (Ok evm') :=
+example (evm:Evm): ∃evm', (eval [Push ns, Push ms, Push ls, Dup_3] evm) = (Ok evm') :=
 by
   let n := u256.from_bytes ns;
   let m := u256.from_bytes ms;
@@ -79,14 +79,19 @@ by
   simp_arith
 
 -- Executing SWAP1 has the right effect
-example (evm:Evm): ∃evm', (eval [Push n, Push m, Swap_1] evm) = (Ok evm') :=
+example (evm:Evm): ∃evm', (eval [Push ns, Push ms, Swap_1] evm) = (Ok evm') :=
 by
+  let n := u256.from_bytes ns;
+  let m := u256.from_bytes ms;
   exists {stack := n::m::evm.stack}
   simp [List.set]
 
 -- Executing SWAP2 has the right effect
-example (evm:Evm): ∃evm', (eval [Push n, Push m, Push l, Swap_2] evm) = (Ok evm') :=
+example (evm:Evm): ∃evm', (eval [Push ns, Push ms, Push ls, Swap_2] evm) = (Ok evm') :=
 by
+  let n := u256.from_bytes ns;
+  let m := u256.from_bytes ms;
+  let l := u256.from_bytes ls;
   exists {stack := n::m::l::evm.stack}
   simp [List.set,eval.reduce]
   simp_arith
